Independence of the length of post

experiment/Experiment.Steel.Repr.M.fst
@@ -298,17 +298,22 @@ let steel_change_vequiv (#vs0 #vs1 : vprop_list) (#opened:Mem.inames) (f : vequi
 (*** [prog_tree] *)
 
 type pre_t = vprop_list
-type post_t (a : Type) = a -> vprop_list
+
+/// With this definition the shape of post (i.e. the length of the list) must be independant of the returned value
+/// ALT: [list (a -> vprop')]
+type post_t (a : Type) = len : nat & (a -> (vs : vprop_list {L.length vs = len}))
+let post_vp (#a : Type) (post : post_t a) : a -> vprop_list = post._2
+
 type req_t (pre : pre_t) = sl_t pre -> prop
-type ens_t (pre : pre_t) (a : Type) (post : post_t a) = sl_t pre -> (x : a) -> sl_t (post x) -> prop
+type ens_t (pre : pre_t) (a : Type) (post : post_t a) = sl_t pre -> (x : a) -> sl_t (post_vp post x) -> prop
 
 type repr_steel_t (a : Type)
        (pre : pre_t) (post : post_t a)
        (req : req_t pre) (ens : ens_t pre a post) : Type
   = unit -> Steel a
-             (vprop_of_list pre) (fun x -> vprop_of_list (post x))
+             (vprop_of_list pre) (fun x -> vprop_of_list (post_vp post x))
              (requires fun h0      -> req (rmem_sels pre h0))
-             (ensures  fun h0 x h1 -> ens (rmem_sels pre h0) x (rmem_sels (post x) h1))
+             (ensures  fun h0 x h1 -> ens (rmem_sels pre h0) x (rmem_sels (post_vp post x) h1))
 
 noeq
 type prog_tree : (a : Type u#a) -> Type u#(max (a+1) 2) =
@@ -336,15 +341,16 @@ noeq
 type tree_cond : (#a : Type u#a) -> (t : prog_tree a) -> (pre : pre_t) -> (post : post_t a) -> Type u#(max (a+1) 2) =
   | TCspec  : (#a : Type u#a) -> (#pre : pre_t) -> (#post : post_t a) -> (#req : req_t pre) -> (#ens : ens_t pre a post) ->
               (pre' : pre_t) -> (post' : post_t a) -> (frame : vprop_list) ->
-              (p0 : vequiv pre' L.(pre @ frame)) -> (p1 : ((x : a) -> vequiv (post x @ frame) (post' x))) ->
+              (p0 : vequiv pre' L.(pre @ frame)) ->
+              (p1 : ((x : a) -> vequiv (post_vp post x @ frame) (post_vp post' x))) ->
               tree_cond (Tspec a pre post req ens) pre' post'
   | TCret   : (#a : Type u#a) -> (#x : a) ->
               (pre : pre_t) -> (post : post_t a) ->
-              (p : vequiv pre (post x)) ->
+              (p : vequiv pre (post_vp post x)) ->
               tree_cond (Tret a x) pre post
   | TCbind  : (#a : Type u#a) -> (#b : Type u#a) -> (#f : prog_tree a) -> (#g : (a -> prog_tree b)) ->
-              (pre : pre_t) -> (itm : (a -> vprop_list)) -> (post : post_t b) ->
-              (cf : tree_cond f pre itm) -> (cg : ((x : a) -> tree_cond (g x) (itm x) post)) ->
+              (pre : pre_t) -> (itm : post_t a) -> (post : post_t b) ->
+              (cf : tree_cond f pre itm) -> (cg : ((x : a) -> tree_cond (g x) (post_vp itm x) post)) ->
               tree_cond (Tbind a b f g) pre post
   | TCbindP : (#a : Type u#a) -> (#b : Type u#a) ->
               (#wp : pure_wp a) -> (#x : (unit -> PURE a wp)) -> (#g : (a -> prog_tree b)) ->
@@ -361,7 +367,7 @@ let return_req (pre : pre_t) : req_t pre
   = fun _ -> True
 
 unfold
-let return_ens (#a : Type) (x : a) (p : a -> vprop_list) : ens_t (p x) a p
+let return_ens (#a : Type) (x : a) (p : post_t a) : ens_t (post_vp p x) a p
   = fun sl0 r sl1 ->
       r == x /\ sl1 == sl0
 
@@ -369,23 +375,23 @@ let return_ens (#a : Type) (x : a) (p : a -> vprop_list) : ens_t (p x) a p
 
 unfold
 let bind_req (#a : Type)
-      (#pre : pre_t) (#itm : a -> vprop_list)
+      (#pre : pre_t) (#itm : post_t a)
       (req_f : req_t pre) (ens_f : ens_t pre a itm)
-      (req_g : (x:a) -> req_t (itm x))
+      (req_g : (x:a) -> req_t (post_vp itm x))
   : req_t pre
   = fun sl0 -> req_f sl0 /\
-      (forall (x : a) (sl1 : sl_t (itm x)) .
+      (forall (x : a) (sl1 : sl_t (post_vp itm x)) .
         ens_f sl0 x sl1 ==> req_g x sl1)
 
 unfold
 let bind_ens (#a : Type) (#b : Type)
-      (#pre : pre_t) (#itm : a -> vprop_list) (#post : post_t b)
+      (#pre : pre_t) (#itm : post_t a) (#post : post_t b)
       (req_f : req_t pre) (ens_f : ens_t pre a itm)
-      (ens_g : (x:a) -> ens_t (itm x) b post)
+      (ens_g : (x:a) -> ens_t (post_vp itm x) b post)
   : ens_t pre b post
   = fun sl0 y sl2 ->
       req_f sl0 /\
-      (exists (x : a) (sl1 : sl_t (itm x)) .
+      (exists (x : a) (sl1 : sl_t (post_vp itm x)) .
         ens_f sl0 x sl1 /\
         ens_g x sl1 y sl2)
 
@@ -429,7 +435,8 @@ and tree_ens (#a : Type u#a) (t : prog_tree a)
   | TCspec #a #pre #post #req #ens  pre' post' frame  p0 p1 ->
              (fun sl0' x sl1' ->
                 let sl0, frame0 = extract_vars_f pre' pre frame p0 sl0' in
-                let sl1, frame1 = extract_vars_f (post' x) (post x) frame (Perm.pequiv_sym (p1 x)) sl1' in
+                let sl1, frame1 = extract_vars_f (post_vp post' x) (post_vp post x) frame
+                                                 (Perm.pequiv_sym (p1 x)) sl1' in
                 frame1 == frame0 /\ ens sl0 x sl1)
   | TCret #a #x  pre post  p ->
              (fun sl0 x' sl1 ->
@@ -462,7 +469,7 @@ let tree_of_steel (#a : Type) (#pre : pre_t) (#post : post_t a) (#req : req_t pr
 let repr_of_steel_steel
       (a : Type) (pre : pre_t) (post : post_t a) (req : req_t pre) (ens : ens_t pre a post)
       (pre' : pre_t) (post' : post_t a) (frame : vprop_list)
-      (p0 : vequiv pre' L.(pre @ frame)) (p1 : ((x : a) -> vequiv (post x @ frame) (post' x)))
+      (p0 : vequiv pre' L.(pre @ frame)) (p1 : ((x : a) -> vequiv (post_vp post x @ frame) (post_vp post' x)))
       ($f : repr_steel_t a pre post req ens)
   : (let c = TCspec #a #pre #post #req #ens pre' post' frame p0 p1 in
      repr_steel_t a pre' post' (tree_req _ c) (tree_ens _ c))
@@ -470,12 +477,13 @@ let repr_of_steel_steel
     (**) steel_change_vequiv p0;
     (**) steel_elim_vprop_of_list_append pre frame;
     let x = f () in
-    (**) steel_intro_vprop_of_list_append (post x) frame;
-    (**) let sl1' = gget (vprop_of_list L.(post x @ frame)) in
+    (**) steel_intro_vprop_of_list_append (post_vp post x) frame;
+    (**) let sl1' = gget (vprop_of_list L.(post_vp post x @ frame)) in
     (**) steel_change_vequiv (p1 x);
-    (**) let sl1'' = gget (vprop_of_list (post' x)) in
-    (**) assert (vpl_sels (post' x) sl1'' == extract_vars (p1 x) (vpl_sels L.(post x @ frame) sl1'));
-    (**) extract_vars_sym_l (p1 x) (vpl_sels L.(post x @ frame) sl1');
+    (**) let sl1'' = gget (vprop_of_list (post_vp post' x)) in
+    (**) assert (vpl_sels (post_vp post' x) sl1''
+    (**)      == extract_vars (p1 x) (vpl_sels L.(post_vp post x @ frame) sl1'));
+    (**) extract_vars_sym_l (p1 x) (vpl_sels L.(post_vp post x @ frame) sl1');
     Steel.Effect.Atomic.return x
 
 [@@ __tree_reduce__]
@@ -494,7 +502,7 @@ let repr_of_steel (#a : Type) (pre : pre_t) (post : post_t a) (req : req_t pre) 
 let return_steel
       (a : Type) (x : a)
       (pre : pre_t) (post : post_t a)
-      (p : vequiv pre (post x))
+      (p : vequiv pre (post_vp post x))
   : (let c = TCret #a #x pre post p in
      repr_steel_t a pre post (tree_req _ c) (tree_ens _ c))
   = fun () ->
@@ -514,56 +522,55 @@ let return (#a : Type) (x :a)
 
 
 let elim_tree_req_bind (#a #b : Type) (f : prog_tree a) (g : a -> prog_tree b)
-      (#pre : pre_t) (#post : post_t b) (#itm : a -> vprop_list)
-      (cf  : tree_cond f pre itm) (cg : (x:a) -> tree_cond (g x) (itm x) post)
+      (#pre : pre_t) (#post : post_t b) (#itm : post_t a)
+      (cf  : tree_cond f pre itm) (cg : (x:a) -> tree_cond (g x) (post_vp itm x) post)
       (sl0 : t_of (vprop_of_list pre))
   : Lemma (requires tree_req _ (TCbind #a #b #f #g pre itm post cf cg) (vpl_sels pre sl0))
           (ensures  tree_req f cf (vpl_sels pre sl0) /\
-                    (forall (x : a) (sl1 : t_of (vprop_of_list (itm x))) .
-                      tree_ens f cf (vpl_sels pre sl0) x (vpl_sels (itm x) sl1) ==>
-                      tree_req (g x) (cg x) (vpl_sels (itm x) sl1)))
+                    (forall (x : a) (sl1 : t_of (vprop_of_list (post_vp itm x))) .
+                      tree_ens f cf (vpl_sels pre sl0) x (vpl_sels (post_vp itm x) sl1) ==>
+                      tree_req (g x) (cg x) (vpl_sels (post_vp itm x) sl1)))
   = assert_norm (tree_req _ (TCbind #a #b #f #g pre itm post cf cg) (vpl_sels pre sl0) == (
       tree_req f cf (vpl_sels pre sl0) /\
-      (forall (x : a) (sl1 : sl_t (itm x)) .
+      (forall (x : a) (sl1 : sl_t (post_vp itm x)) .
          tree_ens f cf (vpl_sels pre sl0) x sl1 ==> tree_req (g x) (cg x) sl1)
     ))
 
 let intro_tree_ens_bind (#a #b : Type) (f : prog_tree a) (g : a -> prog_tree b)
-      (#pre : pre_t) (#post : post_t b) (#itm : a -> vprop_list)
-      (cf  : tree_cond f pre itm) (cg : (x:a) -> tree_cond (g x) (itm x) post)
-      (sl0 : t_of (vprop_of_list pre)) (x : a) (sl1 : t_of (vprop_of_list (itm x)))
-      (y : b) (sl2 : t_of (vprop_of_list (post y)))
+      (#pre : pre_t) (#post : post_t b) (#itm : post_t a)
+      (cf  : tree_cond f pre itm) (cg : (x:a) -> tree_cond (g x) (post_vp itm x) post)
+      (sl0 : t_of (vprop_of_list pre)) (x : a) (sl1 : t_of (vprop_of_list (post_vp itm x)))
+      (y : b) (sl2 : t_of (vprop_of_list (post_vp post y)))
   : Lemma (requires tree_req f cf (vpl_sels pre sl0) /\
-                    tree_ens f cf (vpl_sels pre sl0) x (vpl_sels (itm x) sl1) /\
-                    tree_ens (g x) (cg x) (vpl_sels (itm x) sl1) y (vpl_sels (post y) sl2))
+                    tree_ens f cf (vpl_sels pre sl0) x (vpl_sels (post_vp itm x) sl1) /\
+                    tree_ens (g x) (cg x) (vpl_sels (post_vp itm x) sl1) y (vpl_sels (post_vp post y) sl2))
           (ensures  tree_ens _ (TCbind #a #b #f #g pre itm post cf cg)
-                             (vpl_sels pre sl0) y (vpl_sels (post y) sl2))
+                             (vpl_sels pre sl0) y (vpl_sels (post_vp post y) sl2))
   = assert_norm (tree_ens _ (TCbind #a #b #f #g pre itm post cf cg)
-                          (vpl_sels pre sl0) y (vpl_sels (post y) sl2) == (
+                          (vpl_sels pre sl0) y (vpl_sels (post_vp post y) sl2) == (
       tree_req f cf (vpl_sels pre sl0) /\
-        (exists (x : a) (sl1 : sl_t (itm x)) .
+        (exists (x : a) (sl1 : sl_t (post_vp itm x)) .
           tree_ens f cf (vpl_sels pre sl0) x sl1 /\
-          tree_ens (g x) (cg x) sl1 y (vpl_sels (post y) sl2))
+          tree_ens (g x) (cg x) sl1 y (vpl_sels (post_vp post y) sl2))
     ))
 
 let bind_steel
       (a : Type) (b : Type) (f : prog_tree a) (g : (a -> prog_tree b))
-      (pre : pre_t) (itm : (a -> vprop_list)) (post : post_t b)
-      (cf : tree_cond f pre itm) (cg : ((x : a) -> tree_cond (g x) (itm x) post))
-      (rf : repr_steel_t a pre itm (tree_req f cf) (tree_ens f cf))
-      (rg : (x : a) -> repr_steel_t b (itm x) post (tree_req (g x) (cg x)) (tree_ens (g x) (cg x)))
+      (pre : pre_t) (itm : post_t a) (post : post_t b)
+      (cf : tree_cond f pre itm) (cg : ((x : a) -> tree_cond (g x) (post_vp itm x) post))
+      ($rf : repr_steel_t a pre itm (tree_req f cf) (tree_ens f cf))
+      ($rg : (x : a) -> repr_steel_t b (post_vp itm x) post (tree_req (g x) (cg x)) (tree_ens (g x) (cg x)))
   : (let c = TCbind #a #b #f #g pre itm post cf cg in
      repr_steel_t b pre post (tree_req _ c) (tree_ens _ c))
   = fun () ->
     (**) let sl0 = gget (vprop_of_list pre) in
     (**) elim_tree_req_bind f g cf cg sl0;
     let x = rf () in
-    (**) let sl1 = gget (vprop_of_list (itm x)) in
+    (**) let sl1 = gget (vprop_of_list (post_vp itm x)) in
     let y = rg x () in
-    (**) let sl2 = gget (vprop_of_list (post y)) in
+    (**) let sl2 = gget (vprop_of_list (post_vp post y)) in
     (**) intro_tree_ens_bind f g cf cg sl0 x sl1 y sl2;
     Steel.Effect.Atomic.return y
-
 
 [@@ __tree_reduce__]
 let bind (#a #b : Type)
@@ -572,10 +579,11 @@ let bind (#a #b : Type)
   = {
     repr_tree  = Tbind a b f.repr_tree (fun x -> (g x).repr_tree);
     repr_steel = (fun pre0 post0 c ->
-                    let (TCbind #_ #_ #tf #tg pre itm post cf cg) = c in
+                    let (TCbind #a' #b' #tf #tg pre itm post cf cg) = c in
+                    let rg (x : a) : repr_steel_t b (post_vp itm x) post _ _
+                                   = (g x).repr_steel _ _ (cg x) in
                     U.cast (repr_steel_t b pre0 post0 (tree_req _ c) (tree_ens _ c))
-                           (bind_steel a b tf tg pre itm post cf cg
-                              (f.repr_steel _ _ cf) (fun x -> (g x).repr_steel _ _ (cg x))))
+                           (bind_steel a b tf tg pre itm post cf cg (f.repr_steel _ _ cf) rg))
   }
 
 (* --------------------------- *)
@@ -588,18 +596,32 @@ let read_pre  (r : ref nat) : pre_t
   = [vptr' r full_perm]
 unfold
 let read_post (r : ref nat) : post_t nat
-  = fun _ -> [vptr' r full_perm]
+  = (|1, (fun _ -> [vptr' r full_perm])|)
 let read_req  (r : ref nat) : req_t (read_pre r)
   = fun sl0 -> True
 let read_ens  (r : ref nat) : ens_t (read_pre r) nat (read_post r)
-  = fun sl0 x sl1 -> Dl.index sl1 0 == Dl.index sl0 0 /\ x == Dl.index sl0 0
+  = fun sl0 x sl1 ->
+    assert (L.length (vprop_list_sels_t (post_vp (read_post r) x)) == 1)
+      by T.(trefl ());
+    Dl.index sl1 0 == Dl.index sl0 0 /\ x == Dl.index sl0 0
+
+let steel_read0 (r : ref nat) () :
+  Steel nat (vprop_of_list [vptr' r full_perm]) (fun _ -> vprop_of_list [vptr' r full_perm])
+    (requires fun _ -> True)
+    (ensures fun h0 x h1 -> let sl0 = rmem_sels [vptr' r full_perm] h0 in
+                         let sl1 = rmem_sels [vptr' r full_perm] h1 in
+                         Dl.index sl1 0 == Dl.index sl0 0 /\ x == Dl.index sl0 0)
+  =
+    (**) change_equal_slprop (vprop_of_list [vptr' r full_perm]) (vptr r `star` emp);
+    let x = read r in
+    (**) change_equal_slprop (vptr r `star` emp) (vprop_of_list [vptr' r full_perm]);
+    Steel.Effect.Atomic.return x
 
 let steel_read (r : ref nat)
   : repr_steel_t nat (read_pre r) (read_post r) (read_req r) (read_ens r)
-  = fun () -> (**) change_equal_slprop (vprop_of_list (read_pre r)) (vptr r `star` emp);
-           let x = read r in
-           (**) change_equal_slprop (vptr r `star` emp) (vprop_of_list (read_post r x));
-           Steel.Effect.Atomic.return x
+  = U.cast_by (repr_steel_t nat (read_pre r) (read_post r) (read_req r) (read_ens r))
+            (steel_read0 r)
+            (_ by T.(trefl ()))
 
 unfold let r_read (r : ref nat) : repr nat =
   repr_of_steel (read_pre r) (read_post r) (read_req r) (read_ens r) (steel_read r)
@@ -623,16 +645,31 @@ let normal_spec_steps : list norm_step = [
     delta; iota; zeta; primops
   ]
 
+let normal_read_vp : list norm_step = [
+    delta_only [`%read_pre; `%read_post; `%post_vp; `%L.map; `%L.append; `%L.op_At; `%U.app_on];
+    iota; zeta_full
+  ]
 
 //let _ = fun r ->
 //  assert (print_util (test r).repr_tree) by T.(norm normal_tree_steps; qed ())
 
+let test_equiv (r : ref nat) : vequiv ([vptr' r full_perm]) [vptr' r full_perm] =
+  Perm.id_n 1
+
 unfold
 let test_cond (r : ref nat)
-  : tree_cond (test r).repr_tree [vptr' r full_perm] (fun _ -> [vptr' r full_perm])
-  = TCbind _ (fun _ -> [vptr' r full_perm]) _
-      (TCspec _ _ [] (Perm.id_n 1) (fun (_:nat) -> Perm.id_n 1))
-      (fun _ -> TCret _ _ (Perm.id_n 1))
+  : tree_cond (test r).repr_tree [vptr' r full_perm] (|1, (fun _ -> [vptr' r full_perm])|)
+  = _ by T.(
+    apply (`TCbind);
+     (apply (`(TCspec _ (read_post (`@r)) []));
+       (norm normal_read_vp; exact (`test_equiv (`@r)));
+       (let x = intro () in
+        norm normal_read_vp; (* TODO: @ is not unfolded *)
+        exact (`test_equiv (`@r))));
+     (let x = intro () in
+      apply (`TCret);
+       (norm normal_read_vp; exact (`test_equiv (`@r))));
+  qed ())
 
 //let _ = fun r ->
 //  assert (print_util (tree_req (test r).repr_tree (test_cond r)))
